Logic/Modal/Geach.lean
@@ -1,4 +1,4 @@
-import Logic.Modal.Deduction
+import Logic.Modal.Hilbert
 import Logic.Logic.Kripke.RelItr
 import Logic.Vorspiel.BinaryRelations
 
@@ -14,7 +14,7 @@ namespace GeachConfluent
 
 variable {R : Rel α α}
 
- lemma serial_def : Serial R ↔ (GeachConfluent ⟨0, 0, 1, 1⟩ R) := by simp [GeachConfluent, Serial];
+lemma serial_def : Serial R ↔ (GeachConfluent ⟨0, 0, 1, 1⟩ R) := by simp [GeachConfluent, Serial];
 
 lemma reflexive_def : Reflexive R ↔ (GeachConfluent ⟨0, 0, 1, 0⟩ R) := by simp [GeachConfluent, Reflexive];
 
@@ -77,85 +77,54 @@ end MultiGeachConfluent
 
 
 
-namespace LO.System.Axioms
+namespace LO.Axioms
 
 variable {F : Type*} [LogicalConnective F] [BasicModalLogicalConnective F]
 
-abbrev Geach (l : GeachTaple) (p : F) := ◇^[l.i](□^[l.m]p) ⟶ □^[l.j](◇^[l.n]p)
-
-end LO.System.Axioms
-
-
-namespace LO.Modal
-
-variable {Ax : AxiomSet α}
-
-open System
-
-namespace AxiomSet
-
-abbrev Geach (l : GeachTaple) : AxiomSet α := { Axioms.Geach l p | (p) }
-notation:max "𝗴𝗲(" t ")" => AxiomSet.Geach t
+protected abbrev Geach (t : GeachTaple) (p : F) := ◇^[t.i](□^[t.m]p) ⟶ □^[t.j](◇^[t.n]p)
+abbrev Geach.set (t : GeachTaple) : Set F := { Axioms.Geach t p | (p) }
+notation:max "𝗴𝗲(" t ")" => Geach.set t
 
 namespace Geach
 
-lemma T_def : 𝗴𝗲(⟨0, 0, 1, 0⟩) = (𝗧 : AxiomSet α) := by aesop;
-
-lemma B_def : 𝗴𝗲(⟨0, 1, 0, 1⟩) = (𝗕 : AxiomSet α) := by aesop;
-
-lemma D_def : 𝗴𝗲(⟨0, 0, 1, 1⟩) = (𝗗 : AxiomSet α) := by aesop;
-
-lemma Four_def : 𝗴𝗲(⟨0, 2, 1, 0⟩) = (𝟰 : AxiomSet α) := by aesop;
-
-lemma Five_def : 𝗴𝗲(⟨1, 1, 0, 1⟩) = (𝟱 : AxiomSet α) := by aesop;
-
-lemma Dot2_def : 𝗴𝗲(⟨1, 1, 1, 1⟩) = (.𝟮 : AxiomSet α) := by aesop;
-
-lemma C4_def : 𝗴𝗲(⟨0, 1, 2, 0⟩) = (𝗖𝟰 : AxiomSet α) := by aesop;
-
-lemma CD_def : 𝗴𝗲(⟨1, 1, 0, 0⟩) = (𝗖𝗗 : AxiomSet α) := by aesop;
-
-lemma Tc_def : 𝗴𝗲(⟨0, 1, 0, 0⟩) = (𝗧𝗰 : AxiomSet α) := rfl
+lemma T_def    : 𝗴𝗲(⟨0, 0, 1, 0⟩) = (𝗧 : Set F) := rfl
+lemma B_def    : 𝗴𝗲(⟨0, 1, 0, 1⟩) = (𝗕 : Set F) := rfl
+lemma D_def    : 𝗴𝗲(⟨0, 0, 1, 1⟩) = (𝗗 : Set F) := rfl
+lemma Four_def : 𝗴𝗲(⟨0, 2, 1, 0⟩) = (𝟰 : Set F) := rfl
+lemma Five_def : 𝗴𝗲(⟨1, 1, 0, 1⟩) = (𝟱 : Set F) := rfl
+lemma Dot2_def : 𝗴𝗲(⟨1, 1, 1, 1⟩) = (.𝟮 : Set F) := rfl
+lemma C4_def   : 𝗴𝗲(⟨0, 1, 2, 0⟩) = (𝗖𝟰 : Set F) := rfl
+lemma CD_def   : 𝗴𝗲(⟨1, 1, 0, 0⟩) = (𝗖𝗗 : Set F) := rfl
+lemma Tc_def   : 𝗴𝗲(⟨0, 1, 0, 0⟩) = (𝗧𝗰 : Set F) := rfl
 
 end Geach
 
-class IsGeach (Ax : AxiomSet α) where
+class IsGeach (Ax : Set F) where
   taple : GeachTaple
-  char : Ax = AxiomSet.Geach taple := by rfl
+  char : Ax = 𝗴𝗲(taple) := by rfl
 
-instance : IsGeach (α := α) 𝗧 where taple := ⟨0, 0, 1, 0⟩;
+instance : IsGeach (𝗧 : Set F)  where taple := ⟨0, 0, 1, 0⟩;
+instance : IsGeach (𝗕 : Set F)  where taple := ⟨0, 1, 0, 1⟩;
+instance : IsGeach (𝗗 : Set F)  where taple := ⟨0, 0, 1, 1⟩;
+instance : IsGeach (𝟰 : Set F)  where taple := ⟨0, 2, 1, 0⟩;
+instance : IsGeach (𝟱 : Set F)  where taple := ⟨1, 1, 0, 1⟩;
+instance : IsGeach (.𝟮 : Set F) where taple := ⟨1, 1, 1, 1⟩;
+instance : IsGeach (𝗖𝟰 : Set F) where taple := ⟨0, 1, 2, 0⟩;
+instance : IsGeach (𝗖𝗗 : Set F) where taple := ⟨1, 1, 0, 0⟩;
+instance : IsGeach (𝗧𝗰 : Set F) where taple := ⟨0, 1, 0, 0⟩;
 
-instance : IsGeach (α := α) 𝗕 where taple := ⟨0, 1, 0, 1⟩;
-
-instance : IsGeach (α := α) 𝗗 where taple := ⟨0, 0, 1, 1⟩;
-
-instance : IsGeach (α := α) 𝟰 where taple := ⟨0, 2, 1, 0⟩;
-
-instance : IsGeach (α := α) 𝟱 where taple := ⟨1, 1, 0, 1⟩;
-
-instance : IsGeach (α := α) .𝟮 where taple := ⟨1, 1, 1, 1⟩;
-
-instance : IsGeach (α := α) 𝗖𝟰 where taple := ⟨0, 1, 2, 0⟩;
-
-instance : IsGeach (α := α) 𝗖𝗗 where taple := ⟨1, 1, 0, 0⟩;
-
-instance : IsGeach (α := α) 𝗧𝗰 where taple := ⟨0, 1, 0, 0⟩;
-
-
-def MultiGeach : List GeachTaple → AxiomSet α
+def MultiGeach : List GeachTaple → Set F
   | [] => ∅
-  | x :: xs => (AxiomSet.Geach x) ∪ (AxiomSet.MultiGeach xs)
-notation:max "𝗚𝗲(" l ")" => AxiomSet.MultiGeach l
+  | t :: ts => 𝗴𝗲(t) ∪ (MultiGeach ts)
+notation:max "𝗚𝗲(" ts ")" => MultiGeach ts
 
 namespace MultiGeach
 
-@[simp]
-lemma def_nil : 𝗚𝗲([]) = (∅ : AxiomSet α) := by simp [MultiGeach]
+@[simp] lemma def_nil : 𝗚𝗲([]) = (∅ : Set F) := by simp [MultiGeach]
 
-@[simp]
-lemma iff_cons : 𝗚𝗲(x :: l) = (𝗴𝗲(x) : AxiomSet α) ∪ 𝗚𝗲(l) := by simp only [MultiGeach];
+@[simp] lemma iff_cons : 𝗚𝗲(x :: l) = (𝗴𝗲(x) : Set F) ∪ 𝗚𝗲(l) := by simp only [MultiGeach];
 
-lemma mem (h : x ∈ l) : (𝗴𝗲(x) : AxiomSet α) ⊆ 𝗚𝗲(l) := by
+lemma mem (h : x ∈ l) : (𝗴𝗲(x) : Set F) ⊆ 𝗚𝗲(l) := by
   induction l with
   | nil => contradiction;
   | cons a as ih =>
@@ -164,59 +133,35 @@ lemma mem (h : x ∈ l) : (𝗴𝗲(x) : AxiomSet α) ⊆ 𝗚𝗲(l) := by
     . subst_vars; tauto;
     . apply Set.subset_union_of_subset_right $ ih (by assumption);
 
-/-
-@[simp]
-lemma subset_K {l : List Axioms.Geach.Taple} : (𝗞 : AxiomSet α) ⊆ 𝗚𝗲(l) := by
-  induction l with
-  | nil => simp;
-  | cons a as ih => apply Set.subset_union_of_subset_right ih;
--/
-
-/-
-@[simp]
-lemma subset (h : l₁ ⊆ l₂) : (𝗚𝗲(l₁) : AxiomSet α) ⊆ 𝗚𝗲(l₂) := by
-  induction l₁ generalizing l₂ <;> induction l₂;
-  case nil.nil | cons.nil | nil.cons => simp_all;
-  case cons.cons a as iha b bs ihb =>
-    simp_all;
-    constructor;
-    . cases h.1;
-      . subst_vars; tauto;
-      . apply Set.subset_union_of_subset_right $ mem (by assumption);
-    . simpa using (iha h.2);
--/
-
 end MultiGeach
 
-end AxiomSet
+end LO.Axioms
 
 
-namespace DeductionParameter
+namespace LO.Modal
 
-protected abbrev Geach (l : List GeachTaple) : DeductionParameter α := 𝝂(𝗚𝗲(l))
-notation "𝐆𝐞(" l ")" => DeductionParameter.Geach l
+variable {Ax : Theory α}
+
+open System
+
+protected abbrev Geach (l : List GeachTaple) : Hilbert α := 𝝂(𝗚𝗲(l))
+notation "𝐆𝐞(" l ")" => Modal.Geach l
 
 namespace Geach
 
 end Geach
 
-protected class IsGeach (L : DeductionParameter α) (taples : List GeachTaple) where
-  char : L = 𝐆𝐞(taples) := by aesop;
+protected class Hilbert.IsGeach (L : Hilbert α) (ts : List GeachTaple) where
+  char : L = 𝐆𝐞(ts) := by aesop;
 
-attribute [simp] IsGeach.char
+attribute [simp] Hilbert.IsGeach.char
 
 namespace IsGeach
 
-lemma ax {Λ : DeductionParameter α} [geach : Λ.IsGeach ts] : Ax(Λ) = (𝗞 ∪ 𝗚𝗲(ts)) := by
+lemma ax {Λ : Hilbert α} [geach : Λ.IsGeach ts] : Ax(Λ) = (𝗞 ∪ 𝗚𝗲(ts)) := by
   have e := geach.char;
-  simp [DeductionParameter.Geach] at e;
+  simp [Modal.Geach] at e;
   simp_all;
-
-/-
-instance {L : DeductionParameter α} [geach : L.IsGeach] : L.IsNormal := by
-  rw [geach.char];
-  infer_instance;
--/
 
 instance : 𝐊.IsGeach (α := α) [] where
 
@@ -239,7 +184,5 @@ instance : 𝐊𝐓𝟒𝐁.IsGeach (α := α) [⟨0, 0, 1, 0⟩, ⟨0, 2, 1, 0�
 instance : 𝐓𝐫𝐢𝐯.IsGeach (α := α) [⟨0, 0, 1, 0⟩, ⟨0, 1, 0, 0⟩] where
 
 end IsGeach
-
-end DeductionParameter
 
 end LO.Modal
