Logic/Modal/ModalCompanion/GMT.lean
@@ -10,80 +10,14 @@ open LO.Propositional
 
 variable {α : Type u} [DecidableEq α] [Inhabited α] [Encodable α]
 
-variable {iΛ : Superintuitionistic.DeductionParameter α} {mΛ : DeductionParameter α}
+variable {iΛ : Superintuitionistic.DeductionParameter α} {mΛ : Modal.Hilbert α}
 variable {p q r : Superintuitionistic.Formula α}
-
-lemma axiomTc_GTranslate! [System.K4 mΛ] : mΛ ⊢! pᵍ ⟶ □pᵍ := by
-  induction p using Superintuitionistic.Formula.rec' with
-  | hverum => exact dhyp! (nec! verum!);
-  | hfalsum => simp only [GoedelTranslation, efq!];
-  | hand p q ihp ihq =>
-    simp only [GoedelTranslation];
-    exact imp_trans''! (and_replace! ihp ihq) collect_box_and!
-  | hor p q ihp ihq =>
-    simp only [GoedelTranslation];
-    exact imp_trans''! (or₃''! (imply_left_or'! ihp) (imply_right_or'! ihq)) collect_box_or!
-  | _ => simp only [GoedelTranslation, axiomFour!];
-
-instance [System.S4 mΛ] : System.K4 mΛ where
-
-private lemma provable_efq_of_provable_S4.case_imply₁ [System.K4 mΛ] : mΛ ⊢! (p ⟶ q ⟶ p)ᵍ := by
-  simp only [GoedelTranslation];
-  exact nec! $ imp_trans''! axiomTc_GTranslate! $ axiomK'! $ nec! $ imply₁!;
-
-private lemma provable_efq_of_provable_S4.case_imply₂ [System.S4 mΛ] : mΛ ⊢! ((p ⟶ q ⟶ r) ⟶ (p ⟶ q) ⟶ p ⟶ r)ᵍ := by
-  simp only [GoedelTranslation];
-  apply nec! $ imp_trans''! (imp_trans''! (axiomK'! $ nec! ?b) axiomFour!) $ axiomK'! $ nec! $ imp_trans''! (axiomK'! $ nec! imply₂!) axiomK!;
-  apply provable_iff_provable.mpr;
-  apply deduct_iff.mpr;
-  apply deduct_iff.mpr;
-  have : [pᵍ, pᵍ ⟶ □(qᵍ ⟶ rᵍ)] ⊢[mΛ]! pᵍ := by_axm!;
-  have : [pᵍ, pᵍ ⟶ □(qᵍ ⟶ rᵍ)] ⊢[mΛ]! (pᵍ ⟶ □(qᵍ ⟶ rᵍ)) := by_axm!;
-  have : [pᵍ, pᵍ ⟶ □(qᵍ ⟶ rᵍ)] ⊢[mΛ]! □(qᵍ ⟶ rᵍ) := (by assumption) ⨀ (by assumption);
-  exact axiomT'! this;
-
-private lemma provable_efq_of_provable_S4.case_and₃ [System.K4 mΛ] : mΛ ⊢! (p ⟶ q ⟶ p ⋏ q)ᵍ := by
-  simp only [GoedelTranslation];
-  exact nec! $ imp_trans''! axiomTc_GTranslate! $ axiomK'! $ nec! $ and₃!
-
-private lemma provable_efq_of_provable_S4.case_or₃ [System.K4 mΛ] : mΛ ⊢! (((p ⟶ r) ⟶ (q ⟶ r) ⟶ (p ⋎ q ⟶ r)))ᵍ := by
-  simp only [GoedelTranslation];
-  exact nec! $ imp_trans''! axiomFour! $ axiomK'! $ nec! $ imp_trans''! (axiomK'! $ nec! $ or₃!) axiomK!;
-
-private lemma provable_efq_of_provable_S4.case_neg_equiv [System.K4 mΛ] : mΛ ⊢! (Axioms.NegEquiv p)ᵍ := by
-  simp only [GoedelTranslation];
-  apply and₃'!;
-  . exact nec! $ axiomK'! $ nec! $ and₁'! neg_equiv!;
-  . exact nec! $ axiomK'! $ nec! $ and₂'! neg_equiv!;
-
-open provable_efq_of_provable_S4 in
-lemma provable_efq_of_provable_S4 (h : 𝐈𝐧𝐭 ⊢! p) : 𝐒𝟒 ⊢! pᵍ := by
-  induction h.some with
-  | eaxm ih =>
-    simp_all only [Set.mem_setOf_eq];
-    obtain ⟨p, hp⟩ := ih; subst hp;
-    exact nec! efq!;
-  | mdp hpq hp ihpq ihp =>
-    exact axiomT'! $ axiomK''! (by simpa using ihpq ⟨hpq⟩) $ nec! $ ihp ⟨hp⟩;
-  | and₁ => simp only [GoedelTranslation]; exact nec! and₁!;
-  | and₂ => simp only [GoedelTranslation]; exact nec! and₂!;
-  | or₁ => simp only [GoedelTranslation]; exact nec! or₁!;
-  | or₂ => simp only [GoedelTranslation]; exact nec! or₂!;
-  | verum => apply verum!;
-  | imply₁ => exact case_imply₁;
-  | imply₂ => exact case_imply₂;
-  | and₃ => exact case_and₃;
-  | or₃ => exact case_or₃;
-  | neg_equiv => exact case_neg_equiv;
 
 open Kripke
 
 open LO.Kripke
 open Formula
 
-
--- set_option diagnostics true in
--- set_option diagnostics true
 lemma provable_S4_of_provable_efq : (𝐒𝟒 ⊢! pᵍ) → (𝐈𝐧𝐭 ⊢! p) := by
   contrapose;
   intro h;
@@ -127,15 +61,5 @@ lemma provable_S4_of_provable_efq : (𝐒𝟒 ⊢! pᵍ) → (𝐈𝐧𝐭 ⊢! 
 /-- a.k.a. _Gödel-McKinsey-Tarski Theorem_ -/
 theorem provable_efq_iff_provable_S4 : 𝐈𝐧𝐭 ⊢! p ↔ 𝐒𝟒 ⊢! pᵍ := ⟨provable_efq_of_provable_S4, provable_S4_of_provable_efq⟩
 instance : ModalCompanion (α := α) 𝐈𝐧𝐭 𝐒𝟒 := ⟨provable_efq_iff_provable_S4⟩
-
-
-lemma dp_of_mdp [ModalDisjunctive mΛ] [ModalCompanion iΛ mΛ] [System.S4 mΛ] : iΛ ⊢! p ⋎ q → iΛ ⊢! p ∨ iΛ ⊢! q := by
-    intro hpq;
-    have : mΛ ⊢! □pᵍ ⋎ □qᵍ := or₃'''! (imply_left_or'! axiomTc_GTranslate!) (imply_right_or'! axiomTc_GTranslate!) (by simpa using ModalCompanion.companion.mp hpq);
-    cases ModalDisjunctive.modal_disjunctive this with
-    | inl h => left; exact ModalCompanion.companion.mpr h;
-    | inr h => right; exact ModalCompanion.companion.mpr h;
-
-theorem disjunctive_of_modalDisjunctive [ModalDisjunctive mΛ] [ModalCompanion iΛ mΛ] [System.S4 mΛ] : Disjunctive iΛ := ⟨dp_of_mdp (iΛ := iΛ) (mΛ := mΛ)⟩
 
 end LO.Modal
